\documentclass[11pt,a4paper]{jsarticle}
%
\usepackage{amsmath,amssymb}
\usepackage{bm}
\usepackage{graphicx}
\usepackage{ascmac}
\usepackage{pxfonts}
%
\setlength{\textwidth}{\fullwidth}
\setlength{\textheight}{40\baselineskip}
\addtolength{\textheight}{\topskip}
\setlength{\voffset}{-0.2in}
\setlength{\topmargin}{0pt}
\setlength{\headheight}{0pt}
\setlength{\headsep}{0pt}

\begin{document}
We consider the following continuous-time dynamical system in Ver.\ 1.
\begin{eqnarray}
\frac{\text{d}}{\text{d}t}\begin{bmatrix}
   x(t)\\
   y(t)\\
   \theta(t)
\end{bmatrix}=\begin{bmatrix}
   \cos\theta(t) & 0 \\
   \sin\theta(t) & 0 \\
   0 & 1
\end{bmatrix}\begin{bmatrix}
   u_1(t)\\
   u_2(t)
\end{bmatrix}.
\end{eqnarray}
In this study, we design a digital controller with the sampling period $\Delta\ge0$, that is
\begin{eqnarray}
\begin{bmatrix}
   u_1(t) \\
   u_2(t)
\end{bmatrix}=\begin{bmatrix}
   u_{1,k} \\
   u_{2,k}
\end{bmatrix},\ \forall t\in[k\Delta,(k+1)\Delta).
\end{eqnarray}
It is assumed that the system state at $t=k\Delta$ is $[x_{k}\ y_{k}\ \theta_{k}]^{\top}$.

Then, 
\begin{eqnarray}
\theta_{k+1}=\theta((k+1)\Delta)=\theta_{k}+\int_{k\Delta}^{(k+1)\Delta}u_{2,k}\text{d}t=\theta_{k}+u_{2,k}\Delta.
\end{eqnarray}
Additionally, 
\begin{eqnarray}
x_{k+1}&=&x_{k}+u_{1,k}\int_{k\Delta}^{(k+1)\Delta}\cos\theta(t)\text{d}t,\\
y_{k+1}&=&y_{k}+u_{1,k}\int_{k\Delta}^{(k+1)\Delta}\sin\theta(t)\text{d}t,
\end{eqnarray}
where $\theta(t)=\theta_{k}+u_{2,k}(t-k\Delta),\ t\in[k\Delta,(k+1)\Delta)$.

\begin{enumerate}
\item If $u_{2,k}=0$,
	\begin{eqnarray}
	x_{k+1}&=&x_{k}+u_{1,k}\cos\theta_{k}\Delta,\\
	y_{k+1}&=&y_{k}+u_{1,k}\sin\theta_{k}\Delta,\\
	\theta_{k+1}&=&\theta_{k}.
	\end{eqnarray}
\item If $u_{2,k}\neq0$,
	\begin{eqnarray}
	\int_{k\Delta}^{(k+1)\Delta}\cos(t)\text{d}t&=&\int_{k\Delta}^{(k+1)\Delta}\cos(\theta_{k}+u_{2,k}(t-k\delta)\text{d}t\nonumber\\
	&=&\frac{1}{u_{2,k}}\left[\sin(\theta_{k}+u_{2,k}(t-k\Delta))\right]_{k\Delta}^{(k+1)\Delta}\nonumber\\
	&=&\frac{1}{u_{2,k}}(\sin(\theta_{k}+u_{2,k}\Delta)-\sin\theta_{k}),\nonumber
	\end{eqnarray}
	\begin{eqnarray}
	\int_{k\Delta}^{(k+1)\Delta}\sin(t)\text{d}t&=&\int_{k\Delta}^{(k+1)\Delta}\sin(\theta_{k}+u_{2,k}(t-k\delta)\text{d}t\nonumber\\
	&=&\frac{-1}{u_{2,k}}\left[\cos(\theta_{k}+u_{2,k}(t-k\Delta))\right]_{k\Delta}^{(k+1)\Delta}\nonumber\\
	&=&\frac{-1}{u_{2,k}}(\cos(\theta_{k}+u_{2,k}\Delta)-\cos\theta_{k}),\nonumber
	\end{eqnarray}
	Then, 
	\begin{eqnarray}
	x_{k+1}&=&x_{k}+\frac{u_{1,k}}{u_{2,k}}(\sin(\theta_{k}+u_{2,k}\Delta)-\sin\theta_{k}),\\
	y_{k+1}&=&y_{k}+\frac{u_{1,k}}{u_{2,k}}(\cos\theta_{k}-\cos(\theta_{k}+u_{2,k}\Delta)),\\
	\theta_{k+1}&=&\theta_{k}+u_{2,k}\Delta.
	\end{eqnarray}
	If $u_{2,k}\simeq0$, then, 
	\begin{eqnarray}
	&&\lim_{u_{2,k}\Delta\to0}\frac{\sin(\theta_{k}+u_{2,k}\Delta)-\sin\theta_{k}}{u_{2,k}\Delta}=\cos\theta_{k},\nonumber\\
	&&\lim_{u_{2,k}\Delta\to0}\frac{\cos(\theta_{k}+u_{2,k}\Delta)-\cos\theta_{k}}{u_{2,k}\Delta}=-\sin\theta_{k},\nonumber
	\end{eqnarray}
	In this case, 
	\begin{eqnarray}
	x_{k+1}&=&x_{k}+u_{1,k}\Delta\cos\theta_{k},\\
	y_{k+1}&=&y_{k}+u_{1,k}\Delta\sin\theta_{k},\\
	\theta_{k+1}&=&\theta_{k}+u_{2,k}\Delta.
	\end{eqnarray}
\end{enumerate}
\end{document}